removed axiom caching

SystemE/Tactic/ESmt.lean
@@ -1,90 +1,12 @@
 import Lean
 
 import Smt.Tactic.Smt
-import SystemE.Tactic.EQuery
 import SystemE.Tactic.Attr
-import SystemE.Tactic.Translate
-import Qq
 
 namespace Smt
 
-open Qq
 open Lean hiding Command
-open Elab Tactic Qq
-open Smt Translate Query Reconstruct Util
-
-
-#check prepareSmtQuery
-
-def prepareSmtQuery' (oldExprs : List Expr) (initialState : QueryBuilderM.State := { : QueryBuilderM.State }) (hs : List Expr) (goalType : Expr) (fvNames : Std.HashMap FVarId String) : MetaM (List Command) := do
-  let goalId ← Lean.mkFreshMVarId
-  Lean.Meta.withLocalDeclD goalId.name (mkNot goalType) fun g => do
-    Query.generateQuery' oldExprs initialState g hs fvNames
-
-/- Unsound axiom we use to admit results from the solvers
-   Dangerous!
- -/
-universe u
-
-axiom SMT_VERIF (α : Sort u) (synthetic := false) : α
-
-
-def mkSMT_VERIF (type : Expr) (synthetic : Bool) : MetaM Expr := do
-  let u ← Meta.getLevel type
-  return mkApp2 (mkConst ``SMT_VERIF [u]) type (toExpr synthetic)
-
-
-#check Meta.mkSorry
-
-
-def esmt (oldExprs : List Expr) (st : QueryBuilderM.State) (mv : MVarId) (ac : List Command) (hs : List Expr) (timeout' : Option Nat := none) : MetaM (List MVarId) := mv.withContext do
-  let mv₁ := (← Meta.mkFreshExprMVar (← mv.getType)).mvarId!
-  -- 1. Process the hints passed to the tactic.
-  withProcessedHints mv₁ hs fun mv₂ hs => mv₂.withContext do
-  -- let (hs, mv₂) ← Preprocess.elimIff mv₂ hs
-  mv₂.withContext do
-  let goalType : Q(Prop) ← mv₂.getType
-  -- 2. Generate the SMT query.
-  let (fvNames₁, fvNames₂) ← genUniqueFVarNames
-  -- let (st, _) ← prepareSmtQuery' as (← mv.getType) fvNames₁
-  let cmds ← prepareSmtQuery' oldExprs st hs (← mv₂.getType) fvNames₁
-  let cmds := .setLogic "ALL" :: cmds
-  trace[smt] "goal: {goalType}"
-  trace[smt] "\nquery:\n{Command.cmdsAsQuery (cmds ++ [.checkSat])}"
-  -- parse the commands
-  let time1 ← IO.monoMsNow
-  let query := Command.cmdsAsQuery cmds
-  let time2 ← IO.monoMsNow
-  dbg_trace f!"parsing time: {time2 - time1}"
-  -- 3. Run the solver.
-  let res ← solve query (some 1)
-  let time3 ← IO.monoMsNow
-  dbg_trace f!"solving time: {time3 - time2}"
-  -- 4. Print the result.
-  -- trace[smt] "\nresult: {res}"
-  match res with
-  | .error e =>
-    -- 4a. Print error reason.
-    trace[smt] "\nerror reason:\n{repr e}\n"
-    throwError "unable to prove goal, either it is false or you need to define more symbols with `smt [foo, bar]`"
-  | .ok pf =>
-    -- 4b. Reconstruct proof.
-    let goalType ← mv.getType
-    let lsorry ← mkSMT_VERIF goalType (synthetic := true)
-    mv.assign lsorry
-    return []
-    -- let ctx := { userNames := fvNames₂ }
-    -- let (_, ps, p, hp, mvs) ← reconstructProof pf ctx
-    -- let mv₂ ← mv₂.assert (← mkFreshId) p hp
-    -- let ⟨_, mv₂⟩ ← mv₂.intro1
-    -- let mut gs ← mv₂.apply (← Meta.mkAppOptM ``Prop.implies_of_not_and #[listExpr ps.dropLast q(Prop), goalType])
-    -- mv₂.withContext (gs.forM (·.assumption))
-    -- mv.assign (.mvar mv₁)
-    -- return mvs
-
--- open Lean hiding Command
-open Elab Tactic Qq
-open Smt Translate Query Reconstruct Util
+open Elab Tactic
 
 namespace Tactic
 
@@ -94,17 +16,16 @@ syntax (name := esmt) "esmt" smtHints : tactic
 #check Tactic.evalTactic
 #check Tactic.elabTerm
 
-/-
-  if no hints are given the entire local context is used
--/
+#check smtHintElem
 @[tactic esmt]
 def evalESmt : Tactic := fun stx => withMainContext do
   -- evalTactic (← `(tactic | dsimp at *))
 
-  let ⟨st, oldGoals, cmds⟩ := euclidExtension.getState (← getEnv)
-
   let axioms := euclidExtension.getState (← getEnv)
   let userHints ← elabHints ⟨stx[1]⟩
 
-  let mvs ← Smt.esmt oldGoals st (← Tactic.getMainGoal) [] (userHints) none
-  Tactic.replaceMainGoal mvs
+  let lemmaNames : Array Name := euclidExtension.getState (← getEnv)
+  let axioms : Array (TSyntax `term) := lemmaNames.map (fun x => ⟨mkIdent x⟩)
+  -- Manually build: smt [ax1, ax2, ax3, ...]
+  evalTactic (← `(tactic| smt [$[$axioms:term],*]))
+-- unexpected token ',*'; expected ']'
