Book/Prop01.lean
@@ -14,10 +14,12 @@ theorem proposition_1 : ∀ (a b : Point) (AB : Line),
   ∃ c : Point, |(c─a)| = |(a─b)| ∧ |(c─b)| = |(a─b)| :=
 by
   euclid_intros
-  obtain ⟨BCD, h1⟩ := circle_from_points a b (by esmt [*])
-  obtain ⟨ACE, h2⟩ := circle_from_points b a (by esmt [*])
-  obtain ⟨c, hc⟩ := intersection_circles BCD ACE (by esmt [*])
-  have hBCD := point_on_circle_onlyif a b c BCD (by esmt [*])
+  obtain ⟨BCD, h1⟩ := circle_from_points a b (by esmt (timeout := 100))
+  obtain ⟨ACE, h2⟩ := circle_from_points b a (by esmt)
+  -- euclid_apply proposition_1
+  obtain ⟨c, hc⟩ := intersection_circles BCD ACE (by esmt)
+  have hBCD := point_on_circle_onlyif a b c BCD (by esmt)
+>>>>>>> Stashed changes
   have hACE := point_on_circle_onlyif b a c ACE (by esmt [h1, h2, hc])
   use c
   esmt [h1, h2, hc, hBCD, hACE]
